Port marshal stateless API specs to new goose

new/proof/github_com/tchajed/marshal.v
@@ -1,12 +1,406 @@
-Require Import New.generatedproof.github_com.tchajed.marshal.
-Require Import New.proof.proof_prelude.
-Require Import New.proof.github_com.goose_lang.std.
+From Perennial.Helpers Require Import List ListLen.
 
-Section heap.
-Context `{hG: heapGS Σ, !ffi_semantics _ _}.
-Context `{!goGlobalsGS Σ}.
+(* TODO: might need pure theory from here *)
+(* From Perennial.goose_lang.lib Require Import encoding. *)
 
-#[global]
-Program Instance : IsPkgInit marshal := ltac2:(build_pkg_init ()).
+From New.proof.github_com.goose_lang Require Import primitive.
+From New.proof.github_com.goose_lang Require Import std.
+From New.proof Require Import proof_prelude.
+From New.generatedproof.github_com.tchajed Require Import marshal.
 
-End heap.
+Section goose_lang.
+Context `{hG: heapGS Σ, !ffi_semantics _ _} `{!goGlobalsGS Σ}.
+
+#[global] Program Instance : IsPkgInit marshal := ltac2:(build_pkg_init ()).
+
+Theorem wp_ReadInt tail (s: slice.t) q x :
+  {{{ is_pkg_init marshal ∗ own_slice s q (u64_le x ++ tail) }}}
+    marshal @ "ReadInt" #s
+  {{{ s', RET (#x, #s'); own_slice s' q tail }}}.
+Proof.
+  wp_start as "Hs". wp_auto.
+  (*
+  wp_apply (wp_UInt64Get_unchanged with "Hs").
+  { rewrite /list.untype fmap_app take_app_length' //. len. }
+  iIntros "Hs".
+  wp_apply (wp_SliceSkip_small with "Hs").
+  { len. }
+  iIntros (s') "Hs'". wp_auto. iApply "HΦ".
+  rewrite drop_app_length'; [done|len].
+Qed.
+*)
+Admitted.
+
+Theorem wp_ReadInt32 tail s q (x: u32) :
+  {{{ is_pkg_init marshal ∗ own_slice s q (u32_le x ++ tail) }}}
+    marshal@"ReadInt32" #s
+  {{{ s', RET (#x, #s'); own_slice s' q tail }}}.
+Proof.
+  wp_start as "Hs". wp_auto.
+(*
+  wp_apply (wp_UInt32Get_unchanged with "Hs").
+  { rewrite /list.untype fmap_app take_app_length' //. len. }
+  iIntros "Hs".
+  wp_apply (wp_SliceSkip_small with "Hs").
+  { len. }
+  iIntros (s') "Hs'". wp_auto. iApply "HΦ".
+  rewrite drop_app_length'; [done|len].
+Qed.
+*)
+Admitted.
+
+Theorem wp_ReadBytes s q (len: u64) (head tail : list u8) :
+  length head = uint.nat len →
+  {{{ is_pkg_init marshal ∗ own_slice s q (head ++ tail) }}}
+    marshal@"ReadBytes" #s #len
+  {{{ b s', RET (#b, #s'); own_slice b q head ∗ own_slice s' q tail }}}.
+Proof.
+  iIntros (Hlen). wp_start as "Hs". wp_auto.
+(*
+  iDestruct (own_slice_len with "Hs") as %Hsz.
+  autorewrite with len in Hsz.
+  iDestruct (own_slice_wf with "Hs") as %Hwf.
+  wp_apply (wp_SliceTake).
+  { word. }
+  wp_apply (wp_SliceSkip).
+  { word. }
+  wp_auto.
+  iModIntro.
+  iApply "HΦ".
+  iDestruct (slice_small_split _ len with "Hs") as "[Hs1 Hs2]".
+  { len. }
+  iSplitL "Hs1".
+  - rewrite take_app_length' //.
+  - rewrite drop_app_length' //.
+Qed.
+*)
+Admitted.
+
+Theorem wp_ReadBytesCopy s q (len: u64) (head tail : list u8) :
+  length head = uint.nat len →
+  {{{ is_pkg_init marshal ∗ own_slice s q (head ++ tail) }}}
+    marshal@"ReadBytesCopy" #s #len
+  {{{ b s', RET (#b, #s'); own_slice b (DfracOwn 1) head ∗ own_slice s' q tail }}}.
+Proof.
+  iIntros (Hlen). wp_start as "Hs". wp_auto.
+(*
+  wp_apply wp_NewSlice. iIntros (b) "Hb".
+  iDestruct (own_slice_len with "Hs") as %Hsz.
+  iDestruct (own_slice_wf with "Hs") as %Hwf.
+  rewrite length_app in Hsz.
+  wp_apply wp_SliceTake.
+  { word. }
+  iDestruct (slice_small_split _ len with "Hs") as "[Hs Hsclose]".
+  { rewrite length_app. word. }
+  iDestruct (own_slice_acc with "Hb") as "[Hb Hbclose]".
+  wp_apply (wp_SliceCopy_full with "[$Hs $Hb]").
+  { iPureIntro. len. }
+  iIntros (l) "(%Hl_val & Hs & Hb)".
+  iDestruct (own_slice_combine with "Hs Hsclose") as "Hs".
+  { word. }
+  rewrite take_drop.
+  wp_apply (wp_SliceSkip_small with "Hs").
+  { len. }
+  iIntros (s') "Hs'".
+  wp_auto. iApply "HΦ". iModIntro. iSplitR "Hs'".
+  - iApply "Hbclose". rewrite take_app_length' //.
+  - rewrite drop_app_length' //.
+Qed.
+*)
+Admitted.
+
+Theorem wp_ReadBool s q (bit: u8) (tail: list u8) :
+  {{{ is_pkg_init marshal ∗ own_slice s q (bit :: tail) }}}
+    marshal@"ReadBool" (#s)
+  {{{ (b: bool) s', RET (#b, #s');
+      ⌜b = bool_decide (uint.Z bit ≠ 0)⌝ ∗
+      own_slice s' q tail }}}.
+Proof.
+  wp_start as "Hs". wp_auto.
+(*
+  wp_apply (wp_SliceGet with "[$Hs]"); [ auto | ].
+  iIntros "Hs".
+  wp_auto.
+  wp_apply (wp_SliceSkip_small with "Hs").
+  { len. }
+  iIntros (s') "Hs".
+  wp_auto. iModIntro.
+  iApply "HΦ".
+  iSplit.
+  { iPureIntro. rewrite -bool_decide_not !bool_decide_decide.
+    assert (#bit ≠ #(U8 0) ↔ uint.Z bit ≠ 0).
+    { apply not_iff_compat.
+      split.
+    - inversion 1; subst; auto.
+    - intros H.
+      repeat (f_equal; try word).
+    }
+    destruct (decide _), (decide _); auto; tauto.
+  }
+  iApply "Hs".
+Qed.
+*)
+Admitted.
+
+Lemma drop_succ :
+  forall {A : Type} (l : list A) (x : A) (l' : list A) (n : nat),
+  l !! n = Some x -> drop n l = x :: l' -> drop (S n) l = l'.
+Proof.
+  intros A l x l' n Helem Hd.
+  pose proof drop_S l x n. apply H in Helem. rewrite Helem in Hd.
+  inversion Hd. reflexivity.
+Qed.
+
+Fixpoint encodes {A:Type} (enc : list u8) (xs : list A) (has_encoding : list u8 -> A -> Prop): Prop :=
+  match xs with
+    | [] => enc = []
+    | x :: xs' => exists bs bs', xs = x :: xs' /\ enc = bs ++ bs' /\ has_encoding bs x /\ encodes bs' xs' has_encoding
+  end.
+
+Theorem wp_ReadSlice {X : Type} `{!IntoVal X} {goT: go_type} `{!IntoValTyped X goT}
+  (enc : list u8) (enc_sl : slice.t) (xs : list X) (count : w64)
+  (has_encoding : list u8 -> X -> Prop) (own : val -> X -> dfrac -> iProp Σ) (readOne : func.t)
+  (suffix : list u8) (dq : dfrac) :
+  (forall (v : val) (x : X) (dq : dfrac), own v x dq -∗ ⌜v = to_val x⌝) ->
+  {{{ is_pkg_init marshal ∗
+      "Hsl" ∷ own_slice enc_sl dq (enc ++ suffix) ∗
+      "%Henc" ∷ ⌜encodes enc xs has_encoding⌝ ∗
+      "%Hcount" ∷ ⌜uint.nat count = length xs⌝ ∗
+      "#HreadOne" ∷ ∀ enc' enc_sl' suffix' x,
+      {{{ own_slice enc_sl' dq (enc' ++ suffix') ∗
+          ⌜has_encoding enc' x⌝
+      }}}
+        #readOne (#enc_sl')
+      {{{ (v : val) (suff_sl : slice.t), RET (v, #suff_sl); own v x (DfracOwn 1) ∗
+          own_slice suff_sl dq suffix'
+      }}}
+  }}}
+    marshal @ "ReadSlice" #goT #enc_sl #count #readOne
+  {{{ vals b2, RET (#vals, #b2);
+       own_slice vals (DfracOwn 1) xs ∗
+       own_slice b2 dq suffix
+  }}}.
+Proof.
+  iIntros (Hown_val). wp_start as "Hpre". iNamed "Hpre". wp_auto.
+(*
+  wp_apply (wp_ref_to); first val_ty. iIntros (l__b2) "Henc_sl".
+  wp_auto.
+
+  wp_apply (wp_NewSlice). iIntros (gxs) "Hgxs".
+  wp_apply (wp_ref_to); first val_ty. iIntros (l__xs) "Hxs_sl".
+  wp_auto.
+
+  wp_apply (wp_ref_to); first val_ty. iIntros (l__i) "Hi".
+  wp_auto.
+
+  wp_apply (wp_forUpto'
+              (λ i, ∃ (enc' : list u8) (enc_sl' gxs' : slice.t),
+                   (* Loop Bounds *)
+                   "%Hi_ge" ∷ ⌜0 ≤ uint.nat i⌝ ∗
+                   "%Hi_le" ∷ ⌜uint.nat i <= length xs⌝ ∗
+                   (* Encoding *)
+                   "%H_b2_enc" ∷ ⌜encodes enc' (drop (uint.nat i) xs) has_encoding⌝ ∗
+                   "H_b2_sl" ∷ own_slice enc_sl' dq (enc' ++ suffix) ∗
+                   (* Outside variables *)
+                   "Henc_sl" ∷ l__b2 ↦[slice.T byteT] enc_sl' ∗
+                   "Hxs_sl" ∷ l__xs ↦[slice.T goT] gxs' ∗
+                   "Hxs" ∷ own_slice gxs' goT (DfracOwn 1) (take (uint.nat i) xs)
+              )%I
+              with "[$Hi $Hsl $Henc_sl $Hgxs $Hxs_sl]"
+           ).
+  - iSplit. { word. }
+    iPureIntro.
+    split; first word. split; first word. done.
+  - clear ϕ. iIntros "!>" (i Φ) "[IH (i & %Hle)] HΦ". iNamed "IH".
+    wp_auto. wp_load.
+    assert ((uint.nat i <= length xs)%nat) as Hi_length. { word. }
+    assert ((uint.nat i < length xs)%nat) as Hi_l_ne. { word. }
+    apply drop_lt in Hi_l_ne.
+    unfold encodes in H_b2_enc.
+    destruct (drop (uint.nat i) xs) eqn:Hdrop. { contradiction. }
+    destruct H_b2_enc as (H_b2_bs & H_b2_bs' & H_b2_enc & H_b2_enc' & H_b2_encoding & H_b2_enc_next).
+    rewrite H_b2_enc'. rewrite <- app_assoc.
+    wp_apply ("HreadOne" with "[$H_b2_sl //]").
+    iIntros (??) "(Hown_x & Hsuff_sl)".
+    wp_auto. wp_load.
+    pose proof (Hown_val v x (DfracOwn 1)) as Hto_val.
+    iApply Hto_val in "Hown_x". iDestruct "Hown_x" as "%Hown_x".
+    rewrite Hown_x.
+    wp_apply (wp_SliceAppend with "[$Hxs]"). iIntros (s') "Hs'".
+    wp_store. wp_store.
+
+    iModIntro. iApply "HΦ". iFrame.
+    pose proof (take_drop (uint.nat i) xs) as H_td.
+    rewrite Hdrop in H_td.
+    pose proof (length_take_le xs $ uint.nat i) as H_tl.
+    apply H_tl in Hi_length. symmetry in Hi_length.
+    pose proof (list_lookup_middle (take (uint.nat i) xs) l x $ uint.nat i) as Hmiddle.
+    apply Hmiddle in Hi_length as Hlookup.
+    apply take_S_r in Hlookup as Htake.
+    rewrite H_td in Htake.
+    rewrite <- Htake.
+    replace (uint.nat (w64_word_instance.(word.add) i (W64 1))) with (S (uint.nat i)) by word.
+    iFrame. iPureIntro.
+    split; first word. split; first word.
+    apply drop_succ in Hdrop.
+    + rewrite Hdrop. done.
+    + rewrite <- H_td. done.
+  - iIntros "[Hloop Hi]". iNamed "Hloop".
+    wp_auto. wp_load. wp_load. wp_auto.
+    iModIntro. iApply "HΦ".
+    replace (uint.nat (W64 (length xs))) with (length xs) by word.
+    replace (uint.nat (W64 (length xs))) with (length xs) in H_b2_enc by word.
+    rewrite take_ge; [ | word ].
+    rewrite drop_ge in H_b2_enc; [ | word ].
+    unfold encodes in H_b2_enc. rewrite H_b2_enc. rewrite app_nil_l.
+    iFrame.
+Qed.
+*)
+Admitted.
+
+Local Theorem wp_compute_new_cap (old_cap min_cap : u64) :
+  {{{ is_pkg_init marshal }}}
+    marshal@"compute_new_cap" #old_cap #min_cap
+  {{{ (new_cap : u64), RET #new_cap; ⌜uint.Z min_cap ≤ uint.Z new_cap⌝ }}}.
+Proof.
+  wp_start as "_". wp_auto.
+  case_bool_decide; wp_auto.
+  - iApply "HΦ". word.
+  - iApply "HΦ". word.
+Qed.
+
+Local Theorem wp_reserve s (extra : u64) (vs : list u8) :
+  {{{ is_pkg_init marshal ∗ own_slice s (DfracOwn 1) vs ∗ own_slice_cap w8 s }}}
+    marshal@"reserve" (#s) #extra
+  {{{ s', RET #s';
+      ⌜uint.Z extra ≤ uint.Z (slice.cap_f s') - uint.Z (slice.len_f s')⌝ ∗
+      own_slice s' (DfracOwn 1) vs ∗ own_slice_cap w8 s' }}}.
+Proof.
+  wp_start as "[Hs Hcap]". wp_auto.
+(*
+  iDestruct (own_slice_wf with "Hs") as %Hwf.
+  iDestruct (own_slice_sz with "Hs") as %Hsz.
+  wp_apply wp_slice_len.
+  wp_apply wp_SumAssumeNoOverflow. iIntros (Hsum).
+  wp_auto. wp_apply wp_slice_cap.
+  wp_if_destruct.
+  - (* we have to grow. *)
+    wp_apply wp_slice_cap.
+    wp_apply wp_compute_new_cap.
+    iIntros (new_cap Hcap).
+    wp_apply wp_slice_len.
+    wp_apply wp_new_slice_cap; first done.
+    { word. }
+    iIntros (ptr) "Hnew". wp_auto.
+    iDestruct (slice.own_slice_to_small with "Hs") as "Hs".
+    iDestruct (slice.own_slice_acc with "Hnew") as "[Hnew Hcl]".
+    wp_apply (slice.wp_SliceCopy_full with "[Hnew Hs]").
+    { iFrame. iPureIntro. rewrite list_untype_length Hsz length_replicate //. }
+    iIntros "[_ Hnew]". iDestruct ("Hcl" with "Hnew") as "Hnew".
+    wp_auto. iApply "HΦ". iModIntro. iFrame. iPureIntro. simpl. word.
+  - (* already big enough *)
+    iApply "HΦ". iFrame. word.
+Qed.
+*)
+Admitted.
+
+Theorem wp_WriteInt s x (vs : list u8) :
+  {{{ is_pkg_init marshal ∗ own_slice s (DfracOwn 1) vs ∗ own_slice_cap w8 s }}}
+    marshal@"WriteInt" (#s) #x
+  {{{ s', RET #s'; own_slice s' (DfracOwn 1) (vs ++ u64_le x) ∗ own_slice_cap w8 s' }}}.
+Proof.
+  wp_start as "[Hs Hcap]". wp_auto.
+(*
+  wp_apply (wp_reserve with "Hs"). clear s. iIntros (s) "[% Hs]". wp_auto.
+  iDestruct (own_slice_wf with "Hs") as %Hwf.
+  iDestruct (own_slice_sz with "Hs") as %Hsz.
+  wp_apply wp_slice_len. wp_auto.
+  wp_apply (wp_SliceTake_full_cap with "Hs").
+  { word. }
+  iIntros (ex) "[%Hex Hsl]".
+  set (s' := slice_take _ _).
+  wp_apply wp_SliceSkip.
+  { rewrite /slice_take /=. word. }
+  iDestruct (slice.own_slice_split_acc s.(slice.len_f) with "Hsl") as "[Hsl Hclose]".
+  { len. }
+  wp_apply (wp_UInt64Put with "Hsl").
+  { len. }
+  iIntros "Hsl". iDestruct ("Hclose" with "Hsl") as "Hsl".
+  wp_auto. iApply "HΦ". iModIntro.
+  rewrite /own_slice. iExactEq "Hsl". repeat f_equal.
+  rewrite /list.untype fmap_app. f_equal.
+  { rewrite take_app_length' //. len. }
+  rewrite drop_ge; [|len].
+  by list_simplifier.
+Qed.
+*)
+Admitted.
+
+Theorem wp_WriteInt32 s x (vs : list u8) :
+  {{{ is_pkg_init marshal ∗ own_slice s (DfracOwn 1) vs ∗ own_slice_cap w8 s }}}
+    marshal@"WriteInt32" (#s) #x
+  {{{ s', RET #s'; own_slice s' (DfracOwn 1) (vs ++ u32_le x) ∗ own_slice_cap w8 s ∗ own_slice_cap w8 s ∗ own_slice_cap w8 s ∗ own_slice_cap w8 s ∗ own_slice_cap w8 s ∗ own_slice_cap w8 s ∗ own_slice_cap w8 s ∗ own_slice_cap w8 s }}}.
+Proof.
+  wp_start as "[Hs Hcap]". wp_auto.
+(*
+  wp_apply (wp_reserve with "Hs"). clear s. iIntros (s) "[% Hs]". wp_auto.
+  iDestruct (own_slice_wf with "Hs") as %Hwf.
+  iDestruct (own_slice_sz with "Hs") as %Hsz.
+  wp_apply wp_slice_len. wp_auto.
+  wp_apply (wp_SliceTake_full_cap with "Hs").
+  { word. }
+  iIntros (ex) "[%Hex Hsl]".
+  set (s' := slice_take _ _).
+  wp_apply wp_SliceSkip.
+  { rewrite /slice_take /=. word. }
+  iDestruct (slice.own_slice_split_acc s.(slice.len_f) with "Hsl") as "[Hsl Hclose]".
+  { len. }
+  wp_apply (wp_UInt32Put with "Hsl").
+  { len. }
+  iIntros "Hsl". iDestruct ("Hclose" with "Hsl") as "Hsl".
+  wp_auto. iApply "HΦ". iModIntro.
+  rewrite /own_slice. iExactEq "Hsl". repeat f_equal.
+  rewrite /list.untype fmap_app. f_equal.
+  { rewrite take_app_length' //. len. }
+  rewrite drop_ge; [|len].
+  by list_simplifier.
+Qed.
+*)
+Admitted.
+
+Theorem wp_WriteBytes s (vs : list u8) data_sl q (data : list u8) :
+  {{{ is_pkg_init marshal ∗ own_slice s (DfracOwn 1) vs ∗ own_slice data_sl q data ∗ own_slice_cap w8 data_sl }}}
+    marshal@"WriteBytes" (#s) (#data_sl)
+  {{{ s', RET #s';
+    own_slice s' (DfracOwn 1) (vs ++ data) ∗
+    own_slice_cap w8 s' ∗
+    own_slice data_sl q data
+  }}}.
+Proof.
+  wp_start as "(Hs & Hcap & Hdata)". wp_auto.
+(*
+  wp_apply (wp_SliceAppendSlice with "[$Hs $Hdata]"); first done.
+  iIntros (s') "[Hs' Hdata]".
+  iApply ("HΦ" with "[$]").
+Qed.
+*)
+Admitted.
+
+Theorem wp_WriteBool s (vs: list u8) (b: bool) :
+  {{{ is_pkg_init marshal ∗ own_slice s (DfracOwn 1) vs ∗ own_slice_cap w8 s }}}
+    marshal@"WriteBool" #s #b
+  {{{ s', RET (#s');
+      own_slice s' (DfracOwn 1) (vs ++ [if b then W8 1 else W8 0]) ∗
+      own_slice_cap w8 s'
+   }}}.
+Proof.
+  wp_start as "[Hs Hcap]". wp_auto.
+  destruct b; wp_auto.
+(*
+  - wp_apply (wp_SliceAppend with "Hs"); auto.
+  - wp_apply (wp_SliceAppend with "Hs"); auto.
+Qed.
+*)
+Admitted.
+
+End goose_lang.
